Quicksave Mon May 31 05:12:48 PM EEST 2021

Axioms_Classical.thy
@@ -8,88 +8,83 @@ section \<open>Classical instantiation of registerss\<close>
 *)
 
 theory Axioms_Classical
-  imports Main
+  imports Main HOL.Map
 begin
 
-type_synonym 'a update = \<open>'a rel\<close>
+type_synonym 'a update = \<open>'a \<rightharpoonup> 'a\<close>
 
+typ \<open>int update\<close>
+
+(* TODO: direct instantiation *)
 abbreviation (input) comp_update :: "'a update \<Rightarrow> 'a update \<Rightarrow> 'a update" where
-  "comp_update a b \<equiv> b O a"
+  "comp_update a b \<equiv> a \<circ>\<^sub>m b"
 
 abbreviation (input) id_update :: "'a update" where
-  "id_update \<equiv> Id"
+  "id_update \<equiv> Some"
 
 lemma id_update_left: "comp_update id_update a = a"
-  by (rule R_O_Id)
+  by (auto intro!: ext simp add: map_comp_def option.case_eq_if)
 lemma id_update_right: "comp_update a id_update = a"
-  by (rule Id_O_R)
+  by auto
 
 lemma comp_update_assoc: "comp_update (comp_update a b) c = comp_update a (comp_update b c)"
-  by auto
+  by (auto intro!: ext simp add: map_comp_def option.case_eq_if)
 
 type_synonym ('a,'b) preregister = \<open>'a update \<Rightarrow> 'b update\<close>
 definition preregister :: \<open>('a,'b) preregister \<Rightarrow> bool\<close> where
-  \<open>preregister F \<longleftrightarrow> (\<exists>R. F = Image R)\<close>
+  \<open>preregister F \<longleftrightarrow> (\<exists>g s. \<forall>a m. F a m = (case a (g m) of None \<Rightarrow> None | Some x \<Rightarrow> s x m))\<close>
 
 lemma id_preregister: \<open>preregister id\<close>
   unfolding preregister_def
-  by (metis Image_Id eq_id_iff)
+  apply (rule exI[of _ \<open>\<lambda>m. m\<close>])
+  apply (rule exI[of _ \<open>\<lambda>a m. Some a\<close>])
+  by (simp add: option.case_eq_if)
 
 lemma preregister_mult_right: \<open>preregister (\<lambda>a. comp_update a z)\<close>
   unfolding preregister_def 
-  apply (rule exI[of _ \<open>{((a,b),(c,b))| a b c. (c,a) \<in> z}\<close>])
-  by (auto intro!:ext simp: relcomp_def relcompp_apply Image_def[abs_def])
+  apply (rule exI[of _ \<open>\<lambda>m. the (z m)\<close>])
+  apply (rule exI[of _ \<open>\<lambda>x m. case z m of None \<Rightarrow> None | _ \<Rightarrow> Some x\<close>])
+  by (auto simp add: option.case_eq_if)
 
 lemma preregister_mult_left: \<open>preregister (\<lambda>a. comp_update z a)\<close>
   unfolding preregister_def 
-  apply (rule exI[of _ \<open>{((a,b),(a,d))| a b c d. (b,d) \<in> z}\<close>])
-  by (auto intro!:ext simp: relcomp_def relcompp_apply Image_def[abs_def])
+  apply (rule exI[of _ \<open>\<lambda>m. m\<close>])
+  apply (rule exI[of _ \<open>\<lambda>x m. z x\<close>])
+  by (auto simp add: option.case_eq_if)
 
-definition rel_of_preregister :: \<open>('a,'b) preregister \<Rightarrow> (('a\<times>'a)\<times>('b\<times>'b)) set\<close> where
-  \<open>rel_of_preregister F = (SOME R. F = Image R)\<close>
-
-lemma rel_of_preregister: \<open>preregister F \<Longrightarrow> F = Image (rel_of_preregister F)\<close>
-  unfolding preregister_def rel_of_preregister_def
-  by (metis (mono_tags) someI_ex)
-
-lemma preregister_mono: "preregister F \<Longrightarrow> mono F"
-  by (auto simp: preregister_def mono_def Image_def)
-
-lemma comp_preregister: "preregister F \<Longrightarrow> preregister G \<Longrightarrow> preregister (G \<circ> F)"
-  unfolding preregister_def apply auto
-  apply (rule_tac x=\<open>R O Ra\<close> in exI)
-  by (auto simp: o_def)
-
-lemma converse_preregister: \<open>preregister converse\<close>
-  unfolding preregister_def
-  apply (rule exI[where x=\<open>{((x,y),(y,x))| x y. True}\<close>])
-  by (auto simp: converse_def Image_def)
+lemma comp_preregister: "preregister (G \<circ> F)" if "preregister F" and \<open>preregister G\<close>
+proof -
+  from \<open>preregister F\<close>
+  obtain sF gF where F: \<open>F a m = (case a (gF m) of None \<Rightarrow> None | Some x \<Rightarrow> sF x m)\<close> for a m
+    using preregister_def by blast
+  from \<open>preregister G\<close>
+  obtain sG gG where G: \<open>G a m = (case a (gG m) of None \<Rightarrow> None | Some x \<Rightarrow> sG x m)\<close> for a m
+    using preregister_def by blast
+  define s g where \<open>s a m = (case sF a (gG m) of None \<Rightarrow> None | Some x \<Rightarrow> sG x m)\<close>
+    and \<open>g m = gF (gG m)\<close> for a m
+  have \<open>(G \<circ> F) a m = (case a (g m) of None \<Rightarrow> None | Some x \<Rightarrow> s x m)\<close> for a m
+    unfolding F G s_def g_def
+    by (auto simp add: option.case_eq_if)
+  then show "preregister (G \<circ> F)"
+    using preregister_def by blast
+qed
 
 definition rel_prod :: "('a*'b) set => ('c*'d) set => (('a*'c) * ('b*'d)) set" where
   "rel_prod a b = (\<lambda>((a,b),(c,d)). ((a,c),(b,d))) ` (a \<times> b)"
 
-lemma tensor_update_mult: \<open>rel_prod a b O rel_prod c d = rel_prod (a O c) (b O d)\<close>
-  apply (auto simp: rel_prod_def relcomp_def relcompp_apply case_prod_beta image_def
-      simp flip: Collect_case_prod)
-  by force
+definition tensor_update :: \<open>'a update \<Rightarrow> 'b update \<Rightarrow> ('a\<times>'b) update\<close> where
+  \<open>tensor_update a b m = (case a (fst m) of None \<Rightarrow> None | Some x \<Rightarrow> (case b (snd m) of None \<Rightarrow> None | Some y \<Rightarrow> Some (x,y)))\<close>
 
-
-lemma rel_prod_converse: \<open>(rel_prod a b)\<inverse> = rel_prod (a\<inverse>) (b\<inverse>)\<close>
-  apply (auto simp: rel_prod_def converse_unfold image_def case_prod_beta)
-  by force
-
-lemma rel_prod_Id[simp]: "rel_prod Id Id = Id"
-  by (auto simp: rel_prod_def Id_def case_prod_beta image_def)
-
-abbreviation (input) tensor_update :: \<open>'a update \<Rightarrow> 'b update \<Rightarrow> ('a\<times>'b) update\<close> where
-  \<open>tensor_update \<equiv> rel_prod\<close>
+lemma tensor_update_mult: \<open>comp_update (tensor_update a c) (tensor_update b d) = tensor_update (comp_update a b) (comp_update c d)\<close>
+  by (auto intro!: ext simp add: map_comp_def option.case_eq_if tensor_update_def)
 
 lemma tensor_extensionality:
   assumes \<open>preregister F\<close>
   assumes \<open>preregister G\<close>
   assumes \<open>\<And>a b. F (tensor_update a b) = G (tensor_update a b)\<close>
   shows "F = G"
-proof -
+  sorry (* TODO *)
+(* proof -
   define RF RG where "RF = rel_of_preregister F" and "RG = rel_of_preregister G"
   then have RF: "F = Image RF" and RG: "G = Image RG"
     using rel_of_preregister assms by auto
@@ -116,64 +111,132 @@ proof -
   qed
   then show \<open>F = G\<close>
     using RF RG by simp
-qed
+qed *)
+
+definition "valid_getter_setter g s \<longleftrightarrow> 
+  (\<forall>b. b = s (g b) b) \<and> (\<forall>a b. g (s a b) = a) \<and> (\<forall>a a' b. s a (s a' b) = s a b)"
+
+definition \<open>register_from_getter_setter g s a m = (case a (g m) of None \<Rightarrow> None | Some x \<Rightarrow> Some (s x m))\<close>
+definition \<open>register_apply F a = the o F (Some o a)\<close>
+definition \<open>getter_setter F = (let s = (\<lambda>a. register_apply F (\<lambda>_. a)) in ((\<lambda>m. THE x. s x m = m), s))\<close> for F :: \<open>'a update \<Rightarrow> 'b update\<close>
 
 definition register :: \<open>('a,'b) preregister \<Rightarrow> bool\<close> where
-  \<open>register F \<longleftrightarrow> preregister F \<and> (\<forall>a a'. F a O F a' = F (a O a')) \<and> F Id = Id \<and> (\<forall>a. F (a\<inverse>) = (F a)\<inverse>)\<close>
+  \<open>register F \<longleftrightarrow> (\<exists>g s. F = register_from_getter_setter g s \<and> valid_getter_setter g s)\<close>
 
 lemma register_id: \<open>register F \<Longrightarrow> F id_update = id_update\<close>
-  by (simp add: register_def)
-
-(* lemma preregister_tensor_left: \<open>preregister (\<lambda>a. tensor_update a b)\<close>
-  unfolding preregister_def apply (rule exI[of _ \<open>{((a1,a2),((a1,b1),(a2,b2)))| a1 a2 b1 b2. (b1,b2) \<in> b}\<close>])
-  apply (auto intro!: ext simp: Image_def[abs_def] rel_prod_def case_prod_beta image_def Id_def)
-  by (metis fst_conv snd_conv)
-lemma preregister_tensor_right: \<open>preregister (\<lambda>a. tensor_update b a)\<close>
-  unfolding preregister_def apply (rule exI[of _ \<open>{((a1,a2),((b1,a1),(b2,a2)))| a1 a2 b1 b2. (b1,b2) \<in> b}\<close>])
-  apply (auto intro!: ext simp: Image_def[abs_def] rel_prod_def case_prod_beta image_def Id_def)
-  by (metis fst_conv snd_conv) *)
+  by (auto simp add: register_def valid_getter_setter_def register_from_getter_setter_def)
 
 lemma register_tensor_left: \<open>register (\<lambda>a. tensor_update a id_update)\<close>
-  apply (auto simp: register_def preregister_def)
-    apply (rule exI[of _ \<open>{((a1,a2),((a1,b),(a2,b)))| a1 a2 b. True}\<close>])
-      apply (auto intro!: ext simp: Image_def[abs_def] rel_prod_def case_prod_beta image_def Id_def 
-                  relcompp_apply relcomp_def converse_def)
-  by (metis fst_conv snd_conv)+
+  apply (auto simp: register_def)
+  apply (rule exI[of _ fst])
+  apply (rule exI[of _ \<open>\<lambda>x' (x,y). (x',y)\<close>])
+  by (auto intro!: ext simp add: tensor_update_def valid_getter_setter_def register_from_getter_setter_def option.case_eq_if)
 
 lemma register_tensor_right: \<open>register (\<lambda>a. tensor_update id_update a)\<close>
-  apply (auto simp: register_def preregister_def)
-    apply (rule exI[of _ \<open>{((b1,b2),((a,b1),(a,b2)))| a b1 b2. True}\<close>])
-      apply (auto intro!: ext simp: Image_def[abs_def] rel_prod_def case_prod_beta image_def Id_def 
-                  relcompp_apply relcomp_def converse_def)
-  by (metis fst_conv snd_conv)+
+  apply (auto simp: register_def)
+  apply (rule exI[of _ snd])
+  apply (rule exI[of _ \<open>\<lambda>y' (x,y). (x,y')\<close>])
+  by (auto intro!: ext simp add: tensor_update_def valid_getter_setter_def register_from_getter_setter_def option.case_eq_if)
 
-lemma
-  register_preregister: "register F \<Longrightarrow> preregister F"
-  by (simp add: register_def) 
+lemma register_preregister: "preregister F" if \<open>register F\<close>
+proof -
+  from \<open>register F\<close>
+  obtain s g where F: \<open>F a m = (case a (g m) of None \<Rightarrow> None | Some x \<Rightarrow> Some (s x m))\<close> for a m
+    unfolding register_from_getter_setter_def register_def by blast
+  show ?thesis
+    unfolding preregister_def
+    apply (rule exI[of _ g])
+    apply (rule exI[of _ \<open>\<lambda>x m. Some (s x m)\<close>])
+    using F by simp
+qed
 
-lemma
-  register_comp: "register F \<Longrightarrow> register G \<Longrightarrow> register (G \<circ> F)"  
+lemma register_comp: "register (G \<circ> F)" if \<open>register F\<close> and \<open>register G\<close>
   for F :: "('a,'b) preregister" and G :: "('b,'c) preregister"
-  by (simp add: comp_preregister register_def) 
+proof -
+  from \<open>register F\<close>
+  obtain sF gF where F: \<open>F a m = (case a (gF m) of None \<Rightarrow> None | Some x \<Rightarrow> Some (sF x m))\<close>
+    and validF: \<open>valid_getter_setter gF sF\<close> for a m
+    unfolding register_def register_from_getter_setter_def by blast
+  from \<open>register G\<close>
+  obtain sG gG where G: \<open>G a m = (case a (gG m) of None \<Rightarrow> None | Some x \<Rightarrow> Some (sG x m))\<close>
+    and validG: \<open>valid_getter_setter gG sG\<close> for a m
+    unfolding register_def register_from_getter_setter_def by blast
+  define s g where \<open>s a m = sG (sF a (gG m)) m\<close> and \<open>g m = gF (gG m)\<close> for a m
+  have \<open>(G \<circ> F) a m = (case a (g m) of None \<Rightarrow> None | Some x \<Rightarrow> Some (s x m))\<close> for a m
+    by (auto simp add: option.case_eq_if F G s_def g_def)
+  moreover have \<open>valid_getter_setter g s\<close>
+    using validF validG by (auto simp: valid_getter_setter_def s_def g_def)
+  ultimately show "register (G \<circ> F)"
+    unfolding register_def register_from_getter_setter_def by blast
+qed
 
-lemma
-  register_mult: "register F \<Longrightarrow> comp_update (F a) (F b) = F (comp_update a b)"
-  by (simp add: register_def)
+lemma register_mult: "register F \<Longrightarrow> comp_update (F a) (F b) = F (comp_update a b)"
+  by (auto intro!: ext simp: register_def register_from_getter_setter_def[abs_def] valid_getter_setter_def map_comp_def option.case_eq_if)
 
 definition register_pair ::
   \<open>('a update \<Rightarrow> 'c update) \<Rightarrow> ('b update \<Rightarrow> 'c update) \<Rightarrow> (('a\<times>'b) update \<Rightarrow> 'c update)\<close> where
-  \<open>register_pair F G = Image {(((x1,y1),(x2,y2)),(m1,m3)) | x1 x2 y1 y2 m1 m2 m3.
-      ((x1,x2),(m2,m3)) \<in> rel_of_preregister F \<and> ((y1,y2),(m1,m2)) \<in> rel_of_preregister G}\<close>
+  \<open>register_pair F G = (let (gF, sF) = getter_setter F; (gG, sG) = getter_setter G in
+    register_from_getter_setter (\<lambda>m. (gF m, gG m)) (\<lambda>(a,b) m. sF a (sG b m)))\<close>
 
 lemma register_pair_apply:
   assumes [simp]: \<open>register F\<close> \<open>register G\<close>
   assumes \<open>\<And>a b. comp_update (F a) (G b) = comp_update (G b) (F a)\<close>
   shows \<open>(register_pair F G) (tensor_update a b) = comp_update (F a) (G b)\<close>
 proof -
-  have [simp]: \<open>F a = rel_of_preregister F `` a\<close>
-    by (metis assms(1) register_preregister rel_of_preregister)
-  have [simp]: \<open>G b = rel_of_preregister G `` b\<close>
-    by (metis assms(2) register_preregister rel_of_preregister)
+  obtain gF sF gG sG where gsF: \<open>(gF, sF) = getter_setter F\<close> and gsG: \<open>(gG, sG) = getter_setter G\<close>
+    by (metis surj_pair)
+  then have F: \<open>F = register_from_getter_setter gF sF\<close> and G: \<open>G = register_from_getter_setter gG sG\<close>
+    sorry
+  have FG: "register_pair F G = register_from_getter_setter (\<lambda>m. (gF m, gG m)) (\<lambda>(a, b) m. sF a (sG b m))"
+    unfolding register_pair_def gsF[symmetric] gsG[symmetric] by auto
+  show ?thesis
+  proof (rule ext, rename_tac m)
+    fix m
+    consider (aNone) \<open>a (gF m) = None\<close> | (bNone) \<open>b (gG m) = None\<close>
+      | (some) x y where \<open>a (gF m) = Some x\<close> and \<open>b (gG m) = Some y\<close>
+      by auto
+    then show \<open>register_pair F G (tensor_update a b) m = (F a \<circ>\<^sub>m G b) m\<close>
+    proof cases
+      case aNone
+      then show ?thesis
+        apply (subst (2) F, subst (2) G)
+        apply (auto simp: register_pair_def gsF[symmetric] gsG[symmetric] tensor_update_def[abs_def]
+                    case_prod_beta map_comp_def register_from_getter_setter_def[abs_def])
+    next
+      case bNone
+      then show ?thesis sorry
+    next
+      case some
+      then show ?thesis sorry
+    qed
+  qed
+qed
+
+
+
+
+
+
+
+
+
+
+
+
+
+    
+    
+    
+    
+    
+    
+    
+    apply (subst (2) F, subst (2) G)
+    unfolding 
+    apply (auto intro!:ext simp: case_prod_beta register_pair_def gsF[symmetric] gsG[symmetric] 
+                      register_from_getter_setter_def[abs_def] map_comp_def option.case_eq_if
+                      tensor_update_def)
+    apply (smt (verit, best) F G assms(3) map_comp_def option.case_eq_if option.distinct(1) option.sel register_from_getter_setter_def)
 
   show ?thesis
     unfolding register_pair_def 
